Prove the [genExpr] spec.
Also, fixed what was arguably a (trivial) bug in
[genExpr]: we passed the arguments to a commutative
operator in the opposite of the expected order :P

Also, moved the [genJoin_spec] and [genFlows_spec]
hypotheses farther down, to where they are needed.

ifc-machine/pico/tmu/cmach/CodeGen.v
@@ -138,7 +138,8 @@ Definition genVar {n:nat} (l:LAB n) :=
 Fixpoint genExpr {n:nat} (e: rule_expr n) :=
   match e with
   | L_Var l => genVar l
-  | L_Join e1 e2 => genExpr e1 ++ genExpr e2 ++ genJoin
+  (* NC: push the arguments in reverse order. *)
+  | L_Join e1 e2 => genExpr e2 ++ genExpr e1 ++ genJoin
  end.
 
 Fixpoint genScond {n:nat} (s: rule_scond n) : code :=
